concat but no fold

theories/concat_cost.v
@@ -15,12 +15,12 @@ Section proof.
   Context `{!heapGS Σ} `{!na_invG Σ}.
   Context {π : gname}.
 
-  Theorem dconcat_spec (d1 d2 : val) : forall o1 o2,
-    {{{ IsDeque π o1 d1 ∗ IsDeque π o2 d2 ∗ ⏱ time_for_concat ∗ Token π 0 }}}
+  Theorem dconcat_spec_helper (d1 d2 : val) : forall n o1 o2,
+    {{{ isDeque π n o1 d1 ∗ isDeque π n o2 d2 ∗ ⏱ time_for_concat ∗ Token π n }}}
       dconcat d1 d2
-    {{{ d', RET d'; IsDeque π (o1 ++ o2) d' ∗ Token π 0 }}}.
+    {{{ d', RET d'; isDeque π n (o1 ++ o2) d' ∗ Token π n }}}.
   Proof.
-    iIntros (o1 o2 ψ) "(Hd1 & Hd2 & τ & O) Hψ".
+    iIntros (n o1 o2 ψ) "(Hd1 & Hd2 & τ & O) Hψ".
     rewrite /dconcat /IsDeque.
     wp_pures.
     iDestruct (split_time 1 with "τ") as "[ι τ]". by lia.
@@ -44,13 +44,24 @@ Section proof.
         iApply (persist_structure with "H").
       }
     wp_pures.
-    wp_apply (bsize_better_spec with "Hmd1") as "_".
+    wp_apply (ssref_read π _ (isPersFiveTuple _ _ _) with "[Hℓ2 O]") as "%v'
+      [(%pr2 & %ld2 & %md2 & %rd2 & %sf2 & %prC2 & %ldC2 & %mdC2 & %rdC2 & %sfC2
+            & %kPr2 & %kMd2 & %kSf2 & %ltr2 & %rtr2 & -> & %cfg2
+            & #Hpr2 & #Hld2 & #Hmd2 & #Hrd2 & #Hsf2 & #Hltr2 & #Hrtr2 & %Heq2)
+      O]".
+      { iFrame "#". iFrame.
+        iIntros (v) "H".
+        iApply (persist_structure with "H").
+      }
+    wp_pures.
+    wp_apply (bis_empty_spec with "Hmd1") as "_".
     wp_pures.
     destruct (bool_decide (kMd1 = 0)) eqn:?.
     { (* d1 is suffix only *)
       apply bool_decide_eq_true_1 in Heqb as Heqmd.
-      apply bool_decide_code_true in Heqb as ->.
       wp_pures.
+      admit.
+      (*
       wp_apply (push_whole_spec with "[O]") as "%d' [#Hd' O]".
         { iSplitR. iExact "Hsf1". iFrame. ℓisDeque ℓ2. iExact "Hℓ2". }
       iApply "Hψ".
@@ -62,27 +73,18 @@ Section proof.
       rewrite (nil_length_inv _ (eq_sym H1)) in Heq1 |- *.
       aac_normalise in Heq1.
       rewrite Heq1 //.
+      *)
       }
     apply bool_decide_eq_false_1 in Heqb as Heqmd1.
-    apply bool_decide_code_false in Heqb as ->.
     wp_pures.
-    wp_apply (ssref_read π _ (isPersFiveTuple _ _ _) with "[Hℓ2 O]") as "%v'
-      [(%pr2 & %ld2 & %md2 & %rd2 & %sf2 & %prC2 & %ldC2 & %mdC2 & %rdC2 & %sfC2
-            & %kPr2 & %kMd2 & %kSf2 & %ltr2 & %rtr2 & -> & %cfg2
-            & #Hpr2 & #Hld2 & #Hmd2 & #Hrd2 & #Hsf2 & #Hltr2 & #Hrtr2 & %Heq2)
-      O]".
-      { iFrame "#". iFrame.
-        iIntros (v) "H".
-        iApply (persist_structure with "H").
-      }
-    wp_pures.
-    wp_apply (bsize_better_spec with "Hmd2") as "_".
+    wp_apply (bis_empty_spec with "Hmd2") as "_".
     wp_pures.
     destruct (bool_decide (kMd2 = 0)) eqn:?.
     { (* d2 is suffix only *)
-      apply bool_decide_eq_true_1 in Heqb as Heqmd.
-      apply bool_decide_code_true in Heqb as ->.
+      apply bool_decide_eq_true_1 in Heqb0 as Heqmd.
       wp_pures.
+      admit.
+      (*
       wp_apply (inject_whole_spec with "[O]") as "%d' [#Hd' O]".
         { iSplitR. iExact "Hsf2". iFrame. ℓisDeque ℓ1. iExact "Hℓ1". }
       iApply "Hψ".
@@ -94,30 +96,28 @@ Section proof.
       rewrite (nil_length_inv _ (eq_sym H1)) in Heq2 |- *.
       aac_normalise in Heq2.
       rewrite Heq2 //.
+      *)
     }
-    apply bool_decide_eq_false_1 in Heqb as Heqmd2.
-    apply bool_decide_code_false in Heqb as ->.
+    apply bool_decide_eq_false_1 in Heqb0 as Heqmd2.
     wp_pures.
     inversion cfg1; [exfalso; by apply Heqmd2 |].
     inversion cfg2; [exfalso; by apply Heqmd2 |].
-    change (kPr2 ∈ map S [2; 3; 4; 5]) in H6.
-    apply decrease_in in H6 as (kPr2' & -> & HkPr2').
-    wp_apply (bpop_spec2 with "Hpr2") as "%y %pr1' %oBY (Hpr2' & ->)".
-    wp_pures.
     change (kSf1 ∈ map S [2; 3; 4; 5]) in H0.
     apply decrease_in in H0 as (kSf1' & -> & HkSf1').
-    wp_apply (beject_spec2 with "Hsf1") as "%sf1' %x %oBX (Hsf1' & ->)".
+    wp_apply (beject_spec with "Hsf1") as "%sf1' %x %oBX (Hsf1' & ->)".
     wp_pures.
-    wp_apply (bpush_spec2) as "%bm Hbm".
-      { by iApply empty_is_buffer_at. }
-    wp_apply (bpush_spec2 with "Hbm") as "%md' #Hmd'".
+    change (kPr2 ∈ map S [2; 3; 4; 5]) in H6.
+    apply decrease_in in H6 as (kPr2' & -> & HkPr2').
+    wp_apply (bpop_spec with "Hpr2") as "%y %pr1' %oBY (Hpr2' & ->)".
     wp_pures.
-    wp_apply (partition_buffer_left_better_spec with "[Hsf1']") as "%s1' %s1'' %os1' %os1'' %ks1' %ks1'' (#Hs1' & #Hs1'' & (%Hos1' & %Hos1'' & %Hos1eq))".
+    wp_apply (bdoubleton_spec) as "%md' #Hmd'". { done. }
+    wp_pures.
+    wp_apply (bsplit23l_spec with "[Hsf1']") as "%s1' %s1'' %os1' %os1'' %ks1' %ks1'' (#Hs1' & #Hs1'' & (%Hks1' & %Hks1'' & %Heqos1))".
       { iFrame. iPureIntro. invert_all_in; list_elem_of. }
+    rewrite /atriple_.
     wp_pures.
-    iDestruct (na_own_acc _ _ _ (next_stage 0) with "O") as "[O A]".
+    iDestruct (na_own_acc _ _ _ (next_stage n) with "O") as "[O A]".
     iDestruct (split_time time_for_push with "τ") as "[ι τ]". by lia.
-    rewrite !app_nil_r.
     wp_apply (inject_spec_helper with "[Hld1 ι O]") as "%ld1' [#Hld1' O]".
       { iFrame "#". iFrame. }
     wp_pures.
@@ -125,20 +125,20 @@ Section proof.
     iDestruct (split_time time_for_push with "τ") as "[ι τ]". by lia.
     iDestruct ("A" with "O") as "O".
     wp_apply (wp_strong_mono _ _ _ _ _
-      (λ v, ∃ tr trC, isDeque _ 1 tr v ∗
+      (λ v, ∃ tr trC, isDeque _ (S n) tr v ∗
         ⌜ List.concat trC = List.concat ldC1 ++ mdC1 ++ List.concat rdC1 ++ os1' ++ os1'' ⌝ ∗
-        ([∗list] a;b ∈ trC; tr, ▷ triple π 1 a b) ∗
-        Token π 0)%I
+        ([∗list] a;b ∈ trC; tr, ▷ triple π (S n) a b) ∗
+        Token π n)%I
       with "[O ι]") as "%ld1'' (%tr1' & %trC1' & #Hld1'' & %HtrC1' & #trtrC1' & O)"; try done.
     {
-     wp_apply (bsize_better_spec with "Hs1''") as "_".
+     wp_apply (bis_empty_spec with "Hs1''") as "_".
       wp_pures.
       destruct (bool_decide (ks1'' = 0)) eqn:?.
-      - apply bool_decide_eq_true_1 in Heqb as Heqs1.
-        apply bool_decide_code_true in Heqb as ->.
+      - apply bool_decide_eq_true_1 in Heqb1 as Heqs1.
         wp_pures.
         rewrite Heqs1.
-        iDestruct (empty_buffer_is_empty with "Hs1''") as "->".
+        iDestruct (buffer_length with "Hs1''") as "%Hs1''L".
+        destruct os1''; [| inversion Hs1''L].
         rewrite !app_nil_r.
         iExists (ltr1 ++ ⋅(md1, rd1, s1')%V), (ldC1 ++ ⋅(mdC1 ++ List.concat rdC1 ++ os1')).
         iFrame "#". iFrame.
@@ -158,24 +158,25 @@ Section proof.
             iFrame "#".
             doneR.
             iApply (big_sepL2_mono with "Hrtr1"). by auto.
-      - apply bool_decide_eq_false_1 in Heqb as Heqs1.
-        apply bool_decide_code_false in Heqb as ->.
+      - apply bool_decide_eq_false_1 in Heqb1 as Heqs1.
         wp_pures.
-        iDestruct (na_own_acc _ _ _ (next_stage 0) with "O") as "[O A]".
+        iDestruct (na_own_acc _ _ _ (next_stage n) with "O") as "[O A]".
+        wp_apply (abuffer_spec with "Hs1''") as "%ts1'' #Hts1''".
+          { inversion Hks1''; [lia | list_elem_of]. }
         wp_apply (inject_spec_helper with "[Hld1' ι O]") as "%ld1'' [#Hld1'' O]".
           { iFrame "#". iFrame. }
         iDestruct ("A" with "O") as "O".
-        iExists ((ltr1 ++ ⋅(md1, rd1, s1')%V) ++ ⋅(s1'', NONEV, empty_buffer)%V),
+        iExists ((ltr1 ++ ⋅(md1, rd1, s1')%V) ++ ⋅ts1''%V),
                 ((ldC1 ++ ⋅(mdC1 ++ List.concat rdC1 ++ os1')) ++ ⋅os1'').
         iFrame. iFrame "#".
         iSplitL.
         + iPureIntro. rewrite /= !concat_app /=. aac_reflexivity.
-        + iApply (big_sepL2_app with "[Hltr1]");
-        [ iApply (big_sepL2_app with "[Hltr1]") |].
+        + doneR.
+          iApply (big_sepL2_app with "[Hltr1]").
           * iApply (big_sepL2_mono with "Hltr1"). by auto.
           * simpl. doneR.
-            (* TODO(Juliette): factor out *)
-            rewrite triple_unfold.
+            iNext.
+            rewrite !triple_unfold.
             iExists md1, rd1, s1', mdC1, rdC1, os1', kMd1, ks1', rtr1.
             inversion cfg1; [ rewrite -H3 in H14; lia |].
             iSplitR. iPureIntro.
@@ -185,22 +186,12 @@ Section proof.
             iFrame "#".
             doneR.
             iApply (big_sepL2_mono with "Hrtr1"). by auto.
-          * simpl. doneR.
-            rewrite triple_unfold.
-            iExists s1'', empty, empty_buffer, os1'', [], [], ks1'', 0, [].
-            iSplitR. iPureIntro. constructor; invert_all_in; list_elem_of.
-            iSplitR. done.
-            iFrame "#".
-            iSplitR. isEmptyDeque.
-            iSplitR. rewrite /bufferPre. iSplitL. by iApply empty_is_buffer. done.
-            iNext. doneL.
-            iPureIntro; simpl; aac_reflexivity.
     }
     iModIntro. wp_pures.
-    wp_apply (partition_buffer_right_better_spec with "[Hpr2']") as "%p2' %p2'' %op2' %op2'' %kp2' %kp2'' (#Hp2' & #Hp2'' & (%Hp21' & %Hp2'' & %Hop2eq))".
-      { iFrame. iPureIntro. invert_all_in; list_elem_of. }
+    wp_apply (bsplit23r_spec with "[Hpr2']") as "%p2' %p2'' %op2' %op2'' %kp2' %kp2'' (#Hp2' & #Hp2'' & (%Hp21' & %Hp2'' & %Hop2eq))".
+      { iFrame. iPureIntro. clear HkSf1' Hks1' Hks1''. invert_all_in; list_elem_of. }
     wp_pures.
-    iDestruct (na_own_acc _ _ _ (next_stage 0) with "O") as "[O A]".
+    iDestruct (na_own_acc _ _ _ (next_stage n) with "O") as "[O A]".
     iDestruct (split_time time_for_push with "τ") as "[ι τ]". by lia.
     wp_apply (push_spec_helper with "[Hrd2 ι O]") as "%rd2' [#Hrd2' O]".
     { iFrame "#". iFrame. }
@@ -209,21 +200,21 @@ Section proof.
     wp_bind (if: _ then _ else _)%E.
     iDestruct (split_time time_for_push with "τ") as "[ι τ]". by lia.
     wp_apply (wp_strong_mono _ _ _ _ _
-      (λ v, ∃ tr trC, isDeque _ 1 tr v ∗
+      (λ v, ∃ tr trC, isDeque _ (S n) tr v ∗
         ⌜ List.concat trC = op2' ++ op2'' ++ List.concat ldC2 ++ mdC2 ++ List.concat rdC2 ⌝ ∗
-        ([∗list] a;b ∈ trC; tr, ▷ triple π 1 a b) ∗
-        Token π 0)%I
+        ([∗list] a;b ∈ trC; tr, ▷ triple π (S n) a b) ∗
+        Token π n)%I
       with "[ι O]") as "%rd2'' (%tr2' & %trC2' & #Hrd2'' & %HtrC2' & #trtrC2' & O)"; try done.
     {
-      wp_apply (bsize_better_spec with "Hp2'") as "_".
+      wp_apply (bis_empty_spec with "Hp2'") as "_".
       wp_pures.
       destruct (bool_decide (kp2' = 0)) eqn:?.
-      + apply bool_decide_eq_true_1 in Heqb as Heqp2.
-        apply bool_decide_code_true in Heqb as ->.
+      + apply bool_decide_eq_true_1 in Heqb1 as Heqp2.
         wp_pures.
         iFrame.
         rewrite Heqp2.
-        iDestruct (empty_buffer_is_empty with "Hp2'") as "->".
+        iDestruct (buffer_length with "Hp2'") as "%Hp2'L".
+        destruct op2'; [| inversion Hp2'L].
         rewrite !app_nil_l.
         iExists (⋅(p2'', ld2, md2)%V ++ rtr2), (⋅(op2'' ++ List.concat ldC2 ++ mdC2) ++ rdC2).
         iFrame "#".
@@ -235,44 +226,37 @@ Section proof.
             rewrite triple_unfold.
             iExists p2'', ld2, md2, op2'', ldC2, mdC2, kp2'', kMd2, ltr2.
             inversion cfg2.
+            { iDestruct (buffer_length with "Hpr2") as "%Habsurd". inversion Habsurd. }
             iSplitR. iPureIntro.
             destruct (length ldC2); [apply left_leaning | apply has_child];
-              auto with arith; list_elem_of.
+              try lia; list_elem_of.
             iSplitR. done.
             iFrame "#".
             doneR.
             iApply (big_sepL2_mono with "Hltr2"). by auto.
           -- iApply (big_sepL2_mono with "Hrtr2"). by auto.
-      + apply bool_decide_eq_false_1 in Heqb as Heqp2.
-        apply bool_decide_code_false in Heqb as ->.
+      + apply bool_decide_eq_false_1 in Heqb1 as Heqp2.
         wp_pures.
-        iDestruct (na_own_acc _ _ _ (next_stage 0) with "O") as "[O A]".
+        iDestruct (na_own_acc _ _ _ (next_stage n) with "O") as "[O A]".
+        wp_apply (abuffer_spec with "Hp2'") as "%tp2' #Htp2'".
+          { inversion Hp21'; [lia | list_elem_of]. }
         wp_apply (push_spec_helper with "[Hrd2' ι O]") as "%rd2'' [#Hrd2'' O]".
           { iFrame "#". iFrame. }
         iDestruct ("A" with "O") as "O".
         iFrame.
-        iExists (⋅(p2', NONEV, empty_buffer)%V ++ ⋅(p2'', ld2, md2)%V ++ rtr2),
+        iExists (⋅tp2' ++ ⋅(p2'', ld2, md2)%V ++ rtr2),
                 (⋅op2' ++ ⋅(op2'' ++ concat ldC2 ++ mdC2) ++ rdC2).
         iFrame "#".
         iSplitL.
         * iPureIntro. rewrite !concat_app /=. aac_reflexivity.
-        * iApply (big_sepL2_app with "[Hrtr2]");
-        [| iApply (big_sepL2_app with "[Hrtr2]") ].
+        * doneL.
+          iApply (big_sepL2_app with "[Hrtr2]").
           -- simpl. doneR.
-            rewrite triple_unfold. iNext.
-            iExists p2', empty, empty_buffer, op2', [], [], kp2', 0, [].
-            iSplitR. iPureIntro. constructor; invert_all_in; list_elem_of.
-            iSplitR. done.
-            iFrame "#".
-            iSplitR. isEmptyDeque.
-            iSplitR. rewrite /bufferPre. iSplitL. by iApply empty_is_buffer. done.
-            doneL.
-            iPureIntro; simpl; aac_reflexivity.
-          -- simpl. doneR.
-            (* TODO(Juliette): factor out *)
-            rewrite triple_unfold.
+            iNext.
+            rewrite !triple_unfold.
             iExists p2'', ld2, md2, op2'', ldC2, mdC2, kp2'', kMd2, ltr2.
             inversion cfg2.
+            { iDestruct (buffer_length with "Hpr2") as "%Habsurd". inversion Habsurd. }
             iSplitR. iPureIntro.
             destruct (length ldC2); [apply left_leaning | apply has_child];
               auto with arith; list_elem_of.
@@ -282,10 +266,11 @@ Section proof.
             iApply (big_sepL2_mono with "Hltr2"). by auto.
           -- iApply (big_sepL2_mono with "Hrtr2"). by auto.
     }
+    rewrite /assemble_.
     iModIntro. wp_pures.
-    wp_apply (ssref_alloc π (fiveTuple _ 0 (o1 ++ o2)) with "[τ]") as (ℓ') "Hℓ'".
+    wp_apply (ssref_alloc π (fiveTuple _ n (o1 ++ o2)) with "[τ]") as (ℓ') "Hℓ'".
     { iExists pr1, ld1'', md', rd2'', sf2,
-      prC1, trC1', (⋅x ++ ⋅y), trC2', sfC2,
+      prC1, trC1', (⋅oBX ++ ⋅pr1'), trC2', sfC2,
       kPr1, 2, kSf2, tr1', tr2'.
       iSplitR. done.
       iSplitR. iPureIntro. constructor; list_elem_of.
@@ -294,7 +279,7 @@ Section proof.
       iSplitL. iApply (big_sepL2_mono with "trtrC1'"). by auto.
       iSplitL. iApply (big_sepL2_mono with "trtrC2'"). by auto.
       iPureIntro.
-      rewrite Heq1 Heq2 -Hos1eq -Hop2eq HtrC1' HtrC2'.
+      rewrite Heq1 Heq2 Heqos1 Hop2eq HtrC1' HtrC2'.
       aac_reflexivity.
     }
     wp_pures.
@@ -302,6 +287,13 @@ Section proof.
     iFrame.
     ℓisDeque ℓ'. iExact "Hℓ'".
     Unshelve. all: by auto.
-  Qed.
+  Admitted.
+
+  Definition dconcat_spec d1 d2 : forall o1 o2,
+    {{{ isDeque π 0 o1 d1 ∗ isDeque π 0 o2 d2 ∗ ⏱ time_for_concat ∗ Token π 0 }}}
+      dconcat d1 d2
+    {{{ d', RET d'; IsDeque π (o1 ++ o2) d' ∗ Token π 0 }}}
+  :=
+    dconcat_spec_helper d1 d2 0.
 
 End proof.
